//**** init-ting
#import "@preview/physica:0.9.7": *
#import "chpt-temp.typ": *

#show: thmrules.with(qed-symbol: $square$)
#show: chpt-note.with()

#pagebreak()
= Symmetry and Quantum Mechanics
== Symmetries
We associate a unitary operator $cal(I)$ with some operation like translation. By convention we call these symmetry operators. We have seen that for infinitesimal operations we can write
$
  cal(I) = 1 - (i epsilon)/hbar G
$
with $G$ being the Hermitian generator of $cal(I)$. We suppose $H$ is invariant under $cal(I)$. Then
$
  cal(I)^dagger H cal(I) = H <=> [G, H] = 0
$
by the Heisenberg equation of motion then
$
  dv(G, t) = 0
$
so $G$ is an invariant quantity.

Consider an eigenket of $G$ and let the system be in this eigenket at $t_0$. Then at a later time
$
  ket(g'\,t_0\;t) = U(t,t_0) ket(g')
$
with this also being an eigenket of $G$ since $[G,H] = 0$.

Assume $[H,cal(I)] = 0$ for some symmetry operator. Let $ket(n)$ be an energy eigenket with eigenvalue $E_n$. Then $cal(I) ket(n)$ is also an energy eigenket with the same eigenvalue since
$
  H (cal(I) ket(n)) = cal(I) H ket(n) = E_n (cal(I) ket(n))
$
when $ket(n)$ and $cal(I) ket(n)$ are different states we have degeneracy. Typically $cal(I)$ is continuous meaning all $cal(I) (lambda) ket(n)$ have the same energy.

Consider $[D(R),H]=0$ implying $[bold(J),H]=0$ and $[bold(J)^2,H]=0$. Then we have simultaneous eigenkets $ket(n\;j\,m)$ and as before all states $D(R) ket(n\;j\,m)$ have the same energy. This implies that all $ket(n\;j\,m)$ with different $m$ have the same energy since we can mix $m$ by rotation. Then we have degeneracy $d_m = 2 j + 1$.

== $"SO"(4)$ and $r^(-1)$
The invariant for motion in $r^(-1)$ potentials is the Runge-Lenz vector
$
  bold(M) = (bold(p) times bold(L))/m - (Z e^2)/r bold(x)
$
The symmetry responsible for this invariant is $"SO"(4)$. To show this we start by making the invariant Hermitian
$
  bold(M) = 1/(2 m) (bold(p) times bold(L) - bold(L) times bold(p)) - (Z e^2)/r bold(x)
$
With the Hamiltonian
$
  H = bold(p)^2/(2 m) - (Z e^2)/r
$
we can show
$
  [bold(M), H] = 0
$
so $bold(M)$ is actually invariant. We can also show
$
  bold(L) dot bold(M) = 0";  " bold(M)^2 = 2/m H (bold(L)^2 + hbar^2) + Z^2 e^4
$
To find the symmetry we need to know the algebra of the generators of the symmetry. We already know part of it
$
  [L_i, L_j] = i hbar epsilon_(i j k) L_k
$
and we can show
$
  [M_i, L_j] & = i hbar epsilon_(i j k) M_k \
  [M_i, M_j] & = - i hbar epsilon_(i j k) 2/m H L_k
$
so the algebra is not closed which makes our lives harder. We consider specific bound states. Then the vector space is truncated to only those that are eigenstates of $H$ with $E < 0$. This allows us to replace $H$ by $E$ and the algebra becomes closed. We introduce
$
  bold(N) equiv (- m/(2 E))^(1\/2) bold(M)
$
giving the algebra
$
  [L_i,L_j] & = i hbar epsilon_(i j k) L_k \
  [N_i,L_j] & = i hbar epsilon_(i j k) N_k \
  [N_i,N_j] & = i hbar epsilon_(i j k) L_k
$
Which symmetry operation is then generated by $bold(L)$ and $bold(N)$? The first hint that this corresponds to rotation in four spatial dimension is that we have six generators. To show it is correct we essentially generalize our treatment of $bold(L)$ in three dimensions. We associate $(x, y, z) -> (x_1, x_2, x_3)$ and similarly for $p_i$. We rewrite the three dimensional generators
$
  L_3 & = tilde(L)_(1 2) = x_1 p_2 - x_2 p_1 \
  L_2 & = tilde(L)_(1 3) = x_1 p_3 - x_3 p_1 \
  L_1 & = tilde(L)_(2 3) = x_2 p_3 - x_3 p_2
$
and introduce a fourth spatial dimension $x_4$ together with its conjuagte momentum $p_4$. Then we define
$
  tilde(L)_(1 4) & = x_1 p_4 - x_4 p_1 equiv N_1 \
  tilde(L)_(2 4) & = x_2 p_4 - x_4 p_2 equiv N_2 \
  tilde(L)_(3 4) & = x_3 p_4 - x_4 p_3 equiv N_3
$
these $N_i$ obey the previous algebra.

We can define
$
  bold(I) & equiv (bold(L)+bold(N))/2 \
  bold(K) & equiv (bold(L)-bold(N))/2
$
then
$
  [I_i,I_j] & = i hbar epsilon_(i j k) I_k \
  [K_i,K_j] & = i hbar epsilon_(i j k) K_k \
  [I_i,K_j] & = 0
$
so they obey independent angular momentum algebras! We also have $[bold(I),H] = [bold(K),H] = 0$ so they are conserved. We denote the eigenvalues of $bold(I)^2$ and $bold(K)^2$ by $i(i+1)hbar^2$ and $k(k+1)hbar^2$ respectively. Since $bold(I)^2 - bold(K)^2 = bold(L) dot bold(N) = 0$ then $i = k$ and
$
  bold(I)^2 + bold(K)^2 = 1/2 (bold(L)^2 - m/(2 E) bold(M)^2) => 2 k(k+1) hbar^2 = 1/2 (- hbar^2 - m/(2 E) Z^2 e^4)
$
giving the energy
$
  E = - (m Z^2 e^4)/(2 hbar^2) 1/(2 k +1 )^2
$
which is just the Bohr energy with $n -> 2 k + 1$! The degeneracy then lies in both rotational symmetries from $bold(I)$ and $bold(K)$ meaning $d_n = (2 i +1)(2 k +1) = (2 k +1)^2 = n^2$.

The algebra we found corresponds to $"SO"(4)$ and we have seen we can decompose it as $"SO"(4) tilde.equiv "SO"(2) times "SO"(2)$!

== Parity
Parity is the transformation $"RH-system" <--> "LH-system"$. We treat it like
$
  ket(alpha) -> pi ket(alpha)
$
with $pi$ being the parity operator. We require this satisfies
$
  braket(alpha, pi^dagger bold(x) pi, alpha) = - braket(alpha, bold(x), alpha)
$
which happens when
$
  pi^dagger bold(x) pi = - bold(x) => bold(x) pi = - pi bold(x)
$
so when $bold(x)$ and $pi$ anticommute!

We claim
$
  pi ket(bold(x)') = e^(i delta) ket(- bold(x)')
$
with $delta in RR$. To see this consider
$
  bold(x) pi ket(bold(x)') = - pi bold(x) ket(bold(x)') = (- bold(x)') pi ket(bold(x)')
$
so $pi ket(bold(x)')$ is an eigenket of $bold(x)$ with eigenvalue $- bold(x)'$. So it must be $ket(-bold(x)')$ up to a phase. By convention we take $e^(i delta) = 1$. With this convention $pi^2 ket(bold(x)') = ket(bold(x'))$ so $pi^2 = 1$ meaning
$
  pi^(-1) = pi^dagger = pi
$
so it is Hermitian with eigenvalues $plus.minus 1$.

Consider
$
  pi cal(J) (dd(bold(x)')) &= cal(J) (- dd(bold(x)')) pi \
  pi (1 - (i bold(p) dot dd(bold(x)'))/hbar) pi^dagger &= 1 + (i bold(p) dot dd(bold(x)'))/hbar
$
meaning
$
  {pi, bold(p)} = 0 "or" pi^dagger bold(p) pi = - bold(p)
$
so they anticommute! We also find
$
  [pi, bold(L)] = 0
$
since both $bold(x)$ and $bold(p)$ are odd under parity. To show this is general for $bold(J)$ we note that for $3 times 3$ orthogonal matrices
$
  R^"parity" R^"rotation" = R^"rotation" R^"parity"
$
so they commute due to $pi = - bb(1)$ in Euclidean space. We postulate the same relation
$
  pi D (R) = D (R) pi
$
with
$
  D = 1 - (i bold(J) dot hat(bold(n)) epsilon)/hbar
$
Then it follows that
$
  [pi, bold(J)] = 0 "or" pi^dagger bold(J) pi = bold(J)
$
this implies with the previous that $[pi, bold(S)] = 0$!

To summarize $bold(x)$ and $bold(p)$ are odd while $bold(J)$ is even!

Consider a spinless particle described by $ket(alpha)$ with
$
  psi(bold(x)') = braket(bold(x)', alpha)
$
the space-inverted state is
$
  braket(bold(x)', pi, alpha) = braket(-bold(x)', alpha) = psi(- bold(x)')
$
Assuming $ket(alpha)$ is an eigenket of $pi$ then
$
  pi ket(alpha) = plus.minus ket(alpha)
$
so
$
  braket(bold(x)', pi, alpha) = plus.minus braket(bold(x)', alpha)
$
We find
$
  psi(-bold(x)') = plus.minus psi(bold(x)') cases("even parity", "odd parity")
$

#thm[
  Assume $[H,pi] = 0$ and let $ket(n)$ be a non-degenerate eigenket of $H$ with eigenvalue $E_n$. Then $ket(n)$ is also a parity eigenket.
]
#proof[
  Consider
  $
    ket(alpha) equiv 1/2 (1 plus.minus pi) ket(n)
  $
  then $pi ket(alpha) = plus.minus ket(alpha)$ so $ket(alpha)$ is a parity eigenket. Since $[H,pi]=0$ we have $H ket(alpha) = E_n ket(alpha)$ meaning $ket(alpha)$ is also an energy eigenket with eigenvalue $E_n$. We assumed non-degeneracy so these are the same up to a constant. So $ket(n)$ must be a parity eigenket with $pi ket(n) = plus.minus ket(n)$.
]

This more simply follows immediately since $[H,pi] = 0$ meaning they have simultaneous eigenkets.

Consider two parity eigenstates $ket(alpha)$ and $ket(beta)$ with
$
  pi ket(alpha) & = epsilon_alpha ket(alpha) \
   pi ket(beta) & = epsilon_beta ket(beta)
$
Then
$
  braket(beta, bold(x), alpha) = 0
$
unless $epsilon_alpha = - epsilon_beta$. This is easily shown
$
  braket(beta, bold(x), alpha) = braket(beta, pi^(-1) pi bold(x) pi^(-1) pi, alpha) = epsilon_alpha epsilon_beta (- braket(beta, bold(x), alpha))
$
so operators of odd parity connect states of opposite parity. This is the reason why Laporte's rule is valid
$
  integral psi_beta^* bold(x) psi_alpha dd(tau) = 0
$
if $psi_beta$ and $psi_alpha$ have the same parity (due to Wigner).

Assuming $[H,pi] = 0$ with non-degenerate eigenvalues then $braket(n, bold(x), n) = 0$ since $ket(n)$ has parity identical to itself. The dipole moment is defined as $bold(p) equiv q bold(d) prop bold(x)$ so $braket(n, bold(p), n) = 0$ meaning these states can not hold a dipole moment.

== Symmetry breaking
Consider a double well potential (I & III) with a barrier of $V_0$ (II). We let the middle of the barrier be $x=0$ and the width of the barrier is $2 a$ so III starts at $x = a$. We let each well have width $b$ meaning III ends at $x = a +b$. In I and III we have
$
  - hbar^2/(2 m) dv(psi, x, 2) = E psi => dv(psi, x, 2) = - k^2 psi
$
with
$
  k = sqrt(2 m E)/hbar
$
and in II we have
$
  - hbar^2/(2 m) dv(psi, x, 2) + V_0 psi = E psi => dv(psi, x, 2) = kappa^2 psi
$
with
$
  kappa = sqrt(2 m (V_0-E))/hbar
$
Then in III we have
$
  psi_"III" (x) = A sin[k (x-a-b)]
$
which satisfies
$
  psi_"III" (a+b) = 0
$
while due to the finite barrier
$
  psi_"III" (a) = A sin(-k b) eq.not 0
$
For I we use parity since $V(x)$ is symmetric
$
  psi_"I" = plus.minus psi_"III" (-x)
$
For II we have solutions
$
  "even parity" -> psi_"II"^"s" & = C_s cosh(kappa x) \
   "odd parity" -> psi_"II"^"a" & = C_a sinh(kappa x)
$
Then by continuity
$
  psi_"III" (a) = psi_"II" (a)";   " psi'_"III" (a) = psi'_"II" (a)
$
giving a condition of $k$ and $kappa$
$
  "even parity" -> k cot(k b) & = - kappa tanh(kappa a) \
   "odd parity" -> k cot(k b) & = - kappa coth(kappa a)
$
we find a $dd(E, d: Delta) > 0$ since the RHS differs.

Assuming a large barrier where $E << V_0$ or $1 << kappa a$ we find
$
  "RHS"_s tilde.eq - kappa + 2 kappa e^(-2 kappa a)";   " "RHS"_a tilde.eq - kappa - 2 kappa e^(-2 kappa a)
$
And if the wells were isolated and infinite
$
  sin(k b)=0 => k_0 = (n pi)/b
$
For a large barrier these get perturbed $k = k_0 + epsilon$ for some small $epsilon$. Then
$
  cot(k b) = cot(k_0 b + epsilon b) = cot(n pi + epsilon b) = cot (epsilon b) tilde.eq 1/(epsilon b)
$
so
$
  k cot (k b) tilde.eq k_0/(epsilon b) + underbrace(1/b, tilde 0)
$
which gives
$
  k_0/(epsilon_s b) tilde.eq - kappa + 2 kappa e^(-2 kappa a)";   " k_0/(epsilon_a b) tilde.eq -kappa - 2 kappa e^(-2 kappa a)
$
We solve for $epsilon$
$
  epsilon_(s,a) tilde.eq -k_0/(b kappa) 1/(1 minus.plus 2 e^(-2 kappa a)) tilde.eq -k_0/(b kappa) (1 plus.minus 2 e^(-2kappa a))
$
so
$
  k_a -k_s tilde.eq epsilon_a - epsilon_s tilde.eq (4 k_0)/(b kappa) e^(-2 kappa a)
$
This gives the energy difference
$
  dd(E, d: Delta) & = E_a - E_s tilde.eq hbar^2/(2 m) (k_a^2-k_s^2) \
  & tilde.eq hbar^2/(2 m) 2 k_0 (k_a-k_s) = (4 hbar^2 k_0^2)/(m b kappa) e^(-2 kappa a) = (4 hbar^2 pi^2)/(m b^3 kappa) e^(-2 kappa a)
$
with
$
  kappa tilde.eq sqrt(2m V_0)/hbar
$

Consider the linear combinations
$
  ket(R) & = 1/sqrt(2) (ket(S)+ket(A)) \
  ket(L) & = 1/sqrt(2) (ket(S)-ket(A))
$
which are localized in the right- or left well. By construction
$
  pi ket(S) = ket(S)";  " pi ket(A) = - ket(A)
$
but the new states are not parity eigenstates
$
  pi ket(R) = ket(L)";  " pi ket(L) = ket(R)
$
and they are also not energy eigenstates since we had a $dd(E, d: Delta)$ meaning they are not stationary. We let the system be in $ket(R)$ at $t=0$ then
$
  ket(R\,t_0 =0\;t) &= 1/sqrt(2) (exp((i E_s t)/hbar)ket(S)+exp((i E_a t)/hbar) ket(A)) \
  &= 1/sqrt(2) exp((i E_s t)/hbar) (ket(S)+exp((i (E_a-E_s)t)/hbar) ket(A))
$
so the system is in $ket(L)$ at
$
  t = T/2 = (2 pi hbar)/(2 (E_a-E_s))
$
and back in $ket(R)$ at $t = T$. So it oscillates with
$
  omega =(E_a-E_s)/hbar
$
when $V -> oo$: $E_a-E_s = 0$ so tunneling vanishes and the state does not oscillate $ket(L)<-->ket(R)$. This happens since $ket(S)$ and $ket(A)$ become degenerate energy eigenstates implying they are no longer parity eigenstates. So the ground state is assymmetrical even though the Hamiltonian is symmetric. When energy eigenstates are degenerate they do not necessarily obey the symmetries of the Hamiltonian. This is called spontaneous symmetry breaking!

== Bloch's theorem
Consider the case where we have infinitely many periodic potential wells with
$
  V(x plus.minus a) = V(x)
$
Let $cal(T)(l)$ be the translation operator then
$
  cal(T)^dagger (l) x cal(T)(l) = x + l";   " cal(T) (l) ket(x') = ket(x'+l)
$
or
$
  cal(T)^dagger (a) V(x) cal(T) (a) = V(x+a) = V(x)
$
so $cal(T)^dagger (a) H cal(T) (a) = H$ and since $cal(T)$ is unitary
$
  [H,cal(T)(a)] = 0
$
since $cal(T)$ is not Hermitian its eigenvalues have $abs(lambda) = 1$.

We simplify the problem by approximating our potential as periodic minima seperated by infinite potential walls. Then there is no tunneling so the ground state can be localized to any lattice site or minima. We assume it is localized at the $n$th site
$
  H ket(n) = E_0 ket(n)
$
and $braket(x', n) = 0$ outside the $n$th site. We also have infinite degeneracy since $-oo < n < oo$. We also have symmetry breaking since
$
  cal(T) (a) ket(n) = ket(n+1)
$
so $ket(n)$ is not an eigenstate of $cal(T)(a)$ even though the Hamiltonian is! This is expected since we have infinite degeneracy.

We try to find simultaneous eigenkets of $cal(T)(a)$ and $H$. We claim
$
  ket(theta) equiv sum_(n=-oo)^(oo) e^(i n theta) ket(n)
$
does the job. This is clearly an energy eigenket and
$
  cal(T)(a) ket(theta) = sum_(n=-oo)^oo e^(i n theta) ket(n+1) = sum_(n=-oo)^oo e^(i (n-1) theta) ket(n) = e^(-i theta) ket(theta)
$
so it is a simultaneous eigenket and $E_0 eq.not E_0 (theta)$! Consider a finite barrier height then we expect _leakage_
$
  braket(n', H, n) eq.not 0
$
we assume the tight binding approximation
$
  braket(n', H, n) eq.not 0 "iff" n'= {n,n plus.minus 1}
$
and define
$
  braket(n plus.minus 1, H, n) equiv - Delta
$
which is independent of $n$ due to translational invariance. Then assuming $ket(n)$ is an orthogonal basis we have
$
  H ket(n) = E_0 ket(n) - Delta ket(n+1)- Delta ket(n-1)
$
so $ket(n)$ is no longer an energy eigenket! Consider
$
  ket(theta) = sum_(n=-oo)^oo e^(i n theta) ket(n)
$
this is still an eigenstate of $cal(T) (a)$. For the Hamiltonian consider
$
  H ket(theta) &= H sum_(n=-oo)^oo e^(i n theta) ket(n) \
  &= E_0 sum_(n=-oo)^oo e^(i n theta) ket(n) - Delta underbrace(sum_(n=-oo)^oo e^(i n theta) ket(n+1), e^(-i theta) ket(theta)) - Delta underbrace(sum_(n=-oo)^oo e^(i n theta) ket(n-1), e^(i theta) ket(theta)) \
  &= E_0 sum_(n=-oo)^oo e^(i n theta) ket(n) - Delta (e^(-i theta) + e^(i theta)) sum_(n=-oo)^oo e^(i n theta) ket(n) \
  &= (E_0 - 2 Delta cos theta) underbrace(sum_(n=-oo)^oo e^(i n theta) ket(n), ket(theta))
$
so it is a simultaneous eigenket but now the degeneracy has lifted! Since $E=E(theta)$ with a continuous spectrum between $E_0 plus.minus 2 Delta$.

To see what $theta$ means consider $braket(x', theta)$ and
$
  braket(x', cal(T)(a), theta) & = braket(x'-a, theta) \
                               & = e^(-i theta) braket(x', theta) \
        => braket(x'-a, theta) & = braket(x', theta) e^(-i theta)
$
We then make the ansatz
$
  braket(x', theta) = e^(i k x') u_k (x')
$
with $theta = k a$ and $u_k$ periodic with period $a$. Then
$
  e^(i k(x'-a)) u_k (x'-a) = e^(i k x') u_k (x') e^(-i k a)
$
this satisfies $braket(x'-a, theta) = braket(x', theta) e^(-i theta)$. This is Bloch's theorem. The wavefunction of $ket(theta)$ is an eigenket of $cal(T)(a)$ and can be written as a plane wave $e^(i k x')$ times a periodic modulation with period $a$ as above.

We also found the dispersion relation for the first Brillouin zone $abs(k) <= pi\/a$
$
  E(k) = E_0 - 2 Delta cos(k a)
$
